kernel/include/pebble.h
@@ -207,6 +207,19 @@ void pebble_meta_free(void *v);
 #define PEBBLE_MIN_ALLOC 8            /* Minimum allocation is 1 Token */
 #define PEBBLE_MAX_ALLOC (1024 * 1024 * 1024) /* 1 GiB max single alloc */
 
+/* 
+ * B.E.V.I.S. (Byzantine Energy Verification & Isolation Subsystem)
+ * B.U.T.T.H.E.A.D. (Bandwidth-Utilizing Thermodynamic Token Hardened Economic Allocation Dispatcher)
+ */
+#define POW_OP_ALLOC    1
+#define POW_OP_SPAWN    2
+#define POW_OP_NET_BIND 3
+#define POW_OP_REALTIME 4
+
+int pow_calculate_difficulty(int op_class, ulong magnitude);
+int pow_verify(u64int nonce, u64int context, int required_diff);
+void pow_gate_init(void);
+
 #ifndef ROUNDUP
 #define ROUNDUP(n, sz) (((n) + ((sz) - 1)) & ~((sz) - 1))
 #endif
